More investigations of unions and fabs

progs/verif_union.v
@@ -3,13 +3,68 @@ Require Import VST.progs.union.
 Instance CompSpecs : compspecs. make_compspecs prog. Defined.
 Definition Vprog : varspecs. mk_varspecs prog. Defined.
 
-Definition samerep (v1 v2: val) :=
+Import Memdata.
+
+Lemma decode_float32_int32:
+  forall (bl: list memval) (x: float32),
+ size_chunk Mfloat32 = Z.of_nat (Datatypes.length bl) ->
+ decode_val Mfloat32 bl = Vsingle x ->
+ decode_val Mint32 bl = Vint (Float32.to_bits x).
+Proof.
+intros.
+unfold decode_val,decode_int,rev_if_be in *.
+destruct (proj_bytes bl) eqn:?H.
+inv H0.
+rewrite Float32.to_of_bits. auto.
+inv H0.
+Qed.
+
+
+Lemma NOT_decode_int32_float32:
+ ~ (forall (bl: list memval) (x: float32),
+     size_chunk Mfloat32 = Z.of_nat (Datatypes.length bl) ->
+     decode_val Mint32 bl = Vint (Float32.to_bits x) ->
+     decode_val Mfloat32 bl = Vsingle x).
+Proof.
++
+intro.
+set (x := Float32.zero). (* nothing special about zero, any value would do *)
+set (i := Float32.to_bits x).
+set (bl := [Fragment (Vint i) Q32 3; Fragment (Vint i) Q32 2; Fragment (Vint i) Q32 1; Fragment (Vint i) Q32 0]).
+specialize (H bl x).
+specialize (H (eq_refl _)).
+assert (decode_val Mint32 bl = Vint (Float32.to_bits x)).
+unfold decode_val, bl.
+simpl.
+destruct (Val.eq (Vint i) (Vint i)); [ | congruence].
+destruct (quantity_eq Q32 Q32); [ | congruence].
+simpl.
+reflexivity.
+specialize (H H0).
+clear - H. subst bl i.
+unfold decode_val in H.
+simpl in H. inversion H.
+Qed.
+
+
+Lemma decode_float32_iff_int32:
+  forall (bl: list Memdata.memval) (x: float32),
+ Memdata.size_chunk Mfloat32 = Z.of_nat (Datatypes.length bl) ->
+ (Memdata.decode_val Mfloat32 bl = Vsingle x <->
+   Memdata.decode_val Mint32 bl = Vint (Float32.to_bits x)).
+Proof.
+Admitted.  (* not provable at present; see https://github.com/AbsInt/CompCert/issues/207
+    for a description of how to solve this problem. *)
+
+Definition samerep (ch1 ch2: memory_chunk) (v1 v2: val) :=
+  Memdata.size_chunk ch1 = Memdata.size_chunk ch2 /\
   forall bl: list Memdata.memval,
-   Memdata.decode_val Mfloat32 bl = v1 <-> Memdata.decode_val Mint32 bl = v2.
+   Memdata.size_chunk ch1 = Z.of_nat (length bl) ->
+   (Memdata.decode_val ch1 bl = v1 <-> Memdata.decode_val ch2 bl = v2).
 
 Lemma mapsto_single_int: forall sh v1 v2 p,
   is_single v1 -> is_int I32 Unsigned v2 ->
-  samerep v1 v2 ->
+  samerep Mfloat32 Mint32 v1 v2 ->
   mapsto sh (Tfloat F32 noattr) p v1 = mapsto sh (Tint I32 Unsigned noattr) p v2.
 Proof.
   intros.
@@ -25,8 +80,13 @@ Proof.
     unfold res_predicates.address_mapsto.
     apply predicates_hered.pred_ext'. extensionality phi.
     simpl. apply exists_ext; intro bl.
-    f_equal. f_equal. f_equal.
-    specialize (H1 bl). apply prop_ext. auto.
+    f_equal.
+    apply and_ext'; auto. intro.
+    destruct H1 as [H1' H1].
+    specialize (H1 bl).
+    f_equal.
+    apply prop_ext.
+    apply H1. rewrite H3. reflexivity.
  +
     normalize.
     apply pred_ext. normalize. apply exp_left; intro bl. apply exp_right with bl.
@@ -38,7 +98,7 @@ Qed.
 
 Lemma data_at_single_int: forall sh v1 v2 p1 p2,
   is_single v1 -> is_int I32 Unsigned v2 ->
-  samerep v1 v2 ->
+  samerep Mfloat32 Mint32 v1 v2 ->
   readable_share sh ->
   p1 = p2 ->
   data_at sh (Tfloat F32 noattr) v1 p1 = data_at sh (Tint I32 Unsigned noattr) v2 p2.
@@ -56,13 +116,60 @@ Proof.
     erewrite mapsto_single_int; auto.
 Qed.
 
+Lemma float32_to_bits_abs':
+ forall x,
+  Fappli_IEEE_bits.bits_of_b32 (Fappli_IEEE.Babs 24 128 (fun _ pl => (false,pl)) x) =
+   Z.land (Fappli_IEEE_bits.bits_of_b32 x) (2 ^ 31 - 1).
+Proof.
+intros.
+destruct x,b; try reflexivity.
+* (* nan sign=true *)
+simpl.
+destruct n.
+unfold Fappli_IEEE_bits.join_bits.
+change (0+255) with 255.
+admit.
+* (* nan sign=false*)
+admit.
+* (* finite sign=true *)
+unfold Fappli_IEEE_bits.bits_of_b32, Fappli_IEEE.Babs, Fappli_IEEE_bits.bits_of_binary_float.
+Admitted.
+
+Lemma float32_to_bits_abs: 
+  forall x, Float32.to_bits (Float32.abs x) = Int.and (Float32.to_bits x) (Int.repr (2 ^ 31 - 1)).
+Proof.
+intros.
+Transparent Float32.to_bits.
+unfold Float32.to_bits.
+Opaque Float32.to_bits.
+rewrite and_repr.
+f_equal.
+Transparent Float32.abs.
+unfold Float32.abs.
+Opaque Float32.abs.
+unfold Float32.abs_pl.
+apply float32_to_bits_abs'.
+Qed.
 
 Lemma fabs_float32_lemma:
   forall x: float32,
   exists y: int,
-  samerep (Vsingle x) (Vint y) /\
-  samerep (Vsingle (Float32.abs x)) (Vint (Int.and y (Int.repr 2147483647))).
-Admitted.
+  samerep Mfloat32 Mint32 (Vsingle x) (Vint y) /\
+  samerep Mfloat32 Mint32 (Vsingle (Float32.abs x)) (Vint (Int.and y (Int.repr 2147483647))).
+Proof.
+intros.
+exists (Float32.to_bits x).
+split.
+*
+split; [ reflexivity | ].
+intros.
+apply decode_float32_iff_int32; auto.
+*
+split; [ reflexivity | ].
+intros.
+rewrite <- float32_to_bits_abs.
+apply decode_float32_iff_int32; auto.
+Qed.
 
 Module Single.
 
@@ -116,6 +223,11 @@ Qed.
 End Single.
 
 Module Float.
+
+ (* This experiment shows what kind of error message you get
+   if you put the wrong LOCAL precondition.
+   In fact, Vfloat x is wrong, leading to an unsatisfying precondition,
+   it must be Vsingle. *)
 
 Definition fabs_single_spec :=
  DECLARE _fabs_single
